@prefix owl: <http://www.w3.org/2002/07/owl#> .
@prefix dc11: <http://purl.org/dc/elements/1.1/> .
@prefix dc: <http://purl.org/dc/terms/> .
@prefix rdf: <http://www.w3.org/1999/02/22-rdf-syntax-ns#> .
@prefix rdfs: <http://www.w3.org/2000/01/rdf-schema#> .
@prefix xsd: <http://www.w3.org/2001/XMLSchema#> .
@prefix skos: <http://www.w3.org/2004/02/skos/core#> .
@prefix bfo: <http://purl.obolibrary.org/obo/> .
@prefix cco: <https://www.commoncoreontologies.org/> .
@prefix abi: <http://ontology.naas.ai/abi/> .

<http://ontology.naas.ai/abi/OfferingOntology> a owl:Ontology ;
    owl:versionIRI <https://github.com/jupyter-naas/abi/tree/cli/src/core/modules/abi/ontologies/domain-level/OfferingOntology.ttl> ;
    dc11:contributor "Jeremy Ravenel" , "Maxime Jublou" , "Florent Ravenel" ;
    dc:description "Domain ontology for offering."@en ;
    dc:license "" ;
    dc:title "Offering Ontology" .

#################################################################
#    Classes
#################################################################

abi:Offering a owl:Class ;
    rdfs:subClassOf bfo:BFO_0000016 ;
    rdfs:label "Offering"@en ;
    skos:definition "Products or services that are made available by an organization to satisfy wants or needs."@en ;
    skos:example "Products, services, solutions, etc." ;
    abi:is_curated_in_foundry "enterprise_management_foundry" .

abi:Product a owl:Class ;
    rdfs:subClassOf abi:Offering ;
    rdfs:label "Product"@en ;
    skos:definition "Tangible items that are created, manufactured, or sourced to satisfy a want or need."@en ;
    skos:example "A software product, a physical product, a service, etc." ;
    abi:is_curated_in_foundry "enterprise_management_foundry" .

abi:Service a owl:Class ;
    rdfs:subClassOf abi:Offering ;
    rdfs:label "Service"@en ;
    skos:definition "Intangible activities or benefits provided by one party to another, often to solve a problem or meet a need."@en ;
    skos:example "A software service, a physical service, a service, etc." ;
    abi:is_curated_in_foundry "enterprise_management_foundry" .

abi:Solution a owl:Class ;
    rdfs:subClassOf abi:Offering ;
    rdfs:label "Solution"@en ;
    skos:definition "An integrated combination of products and/or services specifically configured and packaged together to comprehensively address a complex business need or challenge."@en ;
    skos:example "An end-to-end cybersecurity solution combining security software, monitoring services, and consulting"@en ,
                 "A complete digital transformation package with hardware, software and training services"@en ;
    abi:is_curated_in_foundry "enterprise_management_foundry" .

abi:Market a owl:Class ;
    rdfs:subClassOf cco:ont00000853 ;
    rdfs:label "Market"@en ;
    skos:definition "Represents the economic space where buyers and sellers interact to exchange goods, services, or information, typically characterized by supply and demand dynamics."@en ;
    skos:example "The technology market"@en ,
                 "The global oil market"@en ;
    rdfs:comment "A market is an abstract concept used to describe the environment in which trade occurs. As such, it is best represented as a Descriptive Information Content Entity that encompasses the characteristics and dynamics of economic exchanges." ;
    abi:is_curated_in_foundry "enterprise_management_foundry" .

abi:MarketSegment a owl:Class ;
    rdfs:subClassOf abi:Market ;
    rdfs:label "Market Segment"@en ;
    skos:definition "Represents a subset of a market, defined by specific characteristics or criteria that distinguish it from other segments, often based on consumer needs, preferences, or demographics."@en ;
    skos:example "The luxury car segment within the automotive market"@en ,
                 "The millennial smartphone user segment"@en ;
    rdfs:comment "A market segment is a more focused abstraction that describes a particular portion of a market with shared attributes. It is best categorized as a Descriptive Information Content Entity that details the specific traits and preferences of a particular group within the larger market." ;
    abi:is_curated_in_foundry "enterprise_management_foundry" .

#################################################################
#    Object Properties
#################################################################

abi:hasOffering a owl:ObjectProperty ;
    rdfs:subPropertyOf cco:BFO_0000218 ;
    rdfs:domain cco:ont00001180 ;
    rdfs:range abi:Offering ;
    rdfs:label "has_offering"@en ;
    skos:definition "Relates an organization to its offerings (products, services, or solutions)."@en .

abi:isOfferingOf a owl:ObjectProperty ;
    rdfs:subPropertyOf bfo:BFO_0000127 ;
    rdfs:domain abi:Offering ;
    rdfs:range cco:ont00001180 ;
    owl:inverseOf abi:hasOffering ;
    rdfs:label "is_offering_of"@en ;
    skos:definition "Relates offerings back to their providing organization."@en .

abi:hasMarket a owl:ObjectProperty ;
    rdfs:subPropertyOf bfo:BFO_0000218 ;
    rdfs:domain cco:ont00001180 ;
    rdfs:range abi:Market ;
    rdfs:label "has market" ;
    skos:definition "Relates an Organization to its Market." ;
    rdfs:comment "This property connects an organization to its market, indicating the market it operates in." .

abi:isMarketOf a owl:ObjectProperty ;
    rdfs:subPropertyOf bfo:BFO_0000127 ;
    rdfs:domain abi:Market ;
    rdfs:range cco:ont00001180 ;
    owl:inverseOf abi:hasMarket ;
    rdfs:label "is market of" ;
    skos:definition "Relates a Market to the Organization that it belongs to." ;
    rdfs:comment "This property connects a market segment to the organization that it belongs to." .

abi:hasMarketSegment a owl:ObjectProperty ;
    rdfs:subPropertyOf bfo:BFO_0000218 ;
    rdfs:domain abi:Market ;
    rdfs:range abi:MarketSegment ;
    rdfs:label "has market segment" ;
    skos:definition "Relates a Market to its Market Segment." ;
    rdfs:comment "This property connects a market to its market segment, indicating the segment of the market it operates in." .

abi:isMarketSegmentOf a owl:ObjectProperty ;
    rdfs:subPropertyOf bfo:BFO_0000127 ;
    rdfs:domain abi:MarketSegment ;
    rdfs:range abi:Market ;
    owl:inverseOf abi:hasMarketSegment ;
    rdfs:label "is market segment of" ;
    skos:definition "Relates a Market Segment to the Market that it belongs to." ;
    rdfs:comment "This property connects a market segment to the market that it belongs to." .

abi:Targets a owl:ObjectProperty ;
    rdfs:subPropertyOf bfo:BFO_0000218 ;
    rdfs:domain abi:Offering ;
    rdfs:range abi:Market ;
    rdfs:label "targets" ;
    skos:definition "Relates an Offering to the Market/MarketSegment that it targets." ;
    rdfs:comment "This property connects an offering to the market/market segment that it targets." .

abi:isTargetedBy a owl:ObjectProperty ;
    rdfs:subPropertyOf bfo:BFO_0000127 ;
    rdfs:domain abi:Market ;
    rdfs:range abi:Offering ;
    owl:inverseOf abi:TargetsMarket ;
    rdfs:label "is targeted by market" ;
    skos:definition "Relates a Market to the Offering that it targets." ;
    rdfs:comment "This property connects a market to the offering that it targets." .

#################################################################
#    Data Properties
#################################################################

abi:market_share a owl:DatatypeProperty ;
    rdfs:domain abi:Offering ;
    rdfs:range xsd:decimal ;
    rdfs:label "market share" ;
    skos:definition "The market share of the offering." .
