@prefix : <http://ontology.naas.ai/messaging#> .
@prefix dc: <http://purl.org/dc/terms/> .
@prefix owl: <http://www.w3.org/2002/07/owl#> .
@prefix rdf: <http://www.w3.org/1999/02/22-rdf-syntax-ns#> .
@prefix xml: <http://www.w3.org/XML/1998/namespace> .
@prefix xsd: <http://www.w3.org/2001/XMLSchema#> .
@prefix dc11: <http://purl.org/dc/elements/1.1/> .
@prefix rdfs: <http://www.w3.org/2000/01/rdf-schema#> .
@prefix skos: <http://www.w3.org/2004/02/skos/core#> .
@prefix bfo: <http://purl.obolibrary.org/obo/BFO_> .
@prefix iao: <http://purl.obolibrary.org/obo/IAO_> .
@base <http://ontology.naas.ai/messaging> .

<http://ontology.naas.ai/messaging.owl> rdf:type owl:Ontology ;
                                        owl:versionIRI <http://ontology.naas.ai/messaging/2024/messaging-core.ttl> ; #message-core.ttl
                                        owl:imports <http://purl.obolibrary.org/obo/bfo.owl> ;
                                        dc11:contributor "Maxime Jublou" ,
                                                        "Florent Ravenel" ,
                                                        "Jeremy Ravenel" ,
                                                        "Giacomo De Colle" ;
                                        dc:description "A formal ontology of message-based communication processes and roles, extending Basic Formal Ontology (BFO) 2020."@en ;
                                        dc:license <https://creativecommons.org/licenses/by/4.0/> ;
                                        dc:title "Message Communication Ontology" ;
                                        rdfs:comment "This ontology provides a systematic account of messaging entities, roles, and processes in accordance with BFO 2020 design patterns." .

#################################################################
#    Annotation properties
#################################################################

###  http://purl.org/dc/elements/1.1/contributor
dc11:contributor rdf:type owl:AnnotationProperty .


###  http://purl.org/dc/elements/1.1/identifier
dc11:identifier rdf:type owl:AnnotationProperty .


###  http://purl.org/dc/terms/description
dc:description rdf:type owl:AnnotationProperty .


###  http://purl.org/dc/terms/license
dc:license rdf:type owl:AnnotationProperty .


###  http://purl.org/dc/terms/title
dc:title rdf:type owl:AnnotationProperty .


###  http://www.w3.org/2004/02/skos/core#definition
skos:definition rdf:type owl:AnnotationProperty .


###  http://www.w3.org/2004/02/skos/core#example
skos:example rdf:type owl:AnnotationProperty .


###  http://www.w3.org/2004/02/skos/core#scopeNote
skos:scopeNote rdf:type owl:AnnotationProperty .


#################################################################
#    Object Properties
#################################################################

###  http://ontology.naas.ai/messaging#hasContent
<http://ontology.naas.ai/messaging#hasContent> rdf:type owl:ObjectProperty ;
                                               rdfs:domain <http://ontology.naas.ai/messaging#Message> ;
                                               rdfs:range <http://ontology.naas.ai/messaging#MessageContent> ;
                                               dc11:identifier "001-MSG" ;
                                               rdfs:label "has content"@en ;
                                               skos:definition "b has content c =Def b is a message & c is message content & c is the information content entity that b bears"@en ;
                                               skos:example "An email message has content the textual information being communicated; a voice message has content the semantic payload being transmitted"@en .








###  http://ontology.naas.ai/messaging#receives
<http://ontology.naas.ai/messaging#receives> rdf:type owl:ObjectProperty ;
                                             rdfs:domain [ rdf:type owl:Class ;
                                                          owl:intersectionOf ( bfo:0000040
                                                                             [ rdf:type owl:Restriction ;
                                                                               owl:onProperty bfo:0000196 ;
                                                                               owl:someValuesFrom <http://ontology.naas.ai/messaging#MessageReceiverRole>
                                                                             ]
                                                                           )
                                                        ] ;
                                             rdfs:range <http://ontology.naas.ai/messaging#Message> ;
                                             dc11:identifier "004-MSG" ;
                                             rdfs:label "receives"@en ;
                                             skos:definition "a receives m =Def a is an agent & a has some message receiver role & m is a message & a obtains m through participating in a message reception process"@en ;
                                             skos:example "An email recipient receives an email message; a chat participant receives a text message"@en .


###  http://ontology.naas.ai/messaging#transmits
<http://ontology.naas.ai/messaging#transmits> rdf:type owl:ObjectProperty ;
                                              rdfs:domain [ rdf:type owl:Class ;
                                                           owl:intersectionOf ( bfo:0000040
                                                                              [ rdf:type owl:Restriction ;
                                                                                owl:onProperty bfo:0000196 ;
                                                                                owl:someValuesFrom <http://ontology.naas.ai/messaging#MessageSenderRole>
                                                                              ]
                                                                            )
                                                         ] ;
                                              rdfs:range <http://ontology.naas.ai/messaging#Message> ;
                                              dc11:identifier "005-MSG" ;
                                              rdfs:label "transmits"@en ;
                                              skos:definition "a transmits m =Def a is an agent & a has some message sender role & m is a message & a sends m through participating in a message transmission process"@en ;
                                              skos:example "An email sender transmits an email; a broadcaster transmits a radio message"@en .


###  http://ontology.naas.ai/messaging#hasMessageInput
<http://ontology.naas.ai/messaging#hasMessageInput> rdf:type owl:ObjectProperty ;
                                                    rdfs:domain <http://ontology.naas.ai/messaging#MessageReceptionProcess> ;
                                                    rdfs:range <http://ontology.naas.ai/messaging#Message> ;
                                                    dc11:identifier "020-MSG" ;
                                                    rdfs:label "has message input"@en ;
                                                    skos:definition "p has message input m =Def p is a message reception process & m is a message & m is the message that serves as input to p"@en ;
                                                    skos:example "A message reception process has message input the received email; a listening process has message input the spoken message"@en .


###  http://ontology.naas.ai/messaging#hasMessageOutput
<http://ontology.naas.ai/messaging#hasMessageOutput> rdf:type owl:ObjectProperty ;
                                                     rdfs:domain <http://ontology.naas.ai/messaging#MessageTransmissionProcess> ;
                                                     rdfs:range <http://ontology.naas.ai/messaging#Message> ;
                                                     dc11:identifier "021-MSG" ;
                                                     rdfs:label "has message output"@en ;
                                                     skos:definition "p has message output m =Def p is a message transmission process & m is a message & m is the message that p produces as output"@en ;
                                                     skos:example "A message transmission process has message output the sent email; a broadcasting process has message output the transmitted signal"@en .


###  http://ontology.naas.ai/messaging#triggeredBy
<http://ontology.naas.ai/messaging#triggeredBy> rdf:type owl:ObjectProperty ;
                                                rdfs:domain <http://ontology.naas.ai/messaging#ResponseGenerationProcess> ;
                                                rdfs:range <http://ontology.naas.ai/messaging#MessageReceptionProcess> ;
                                                dc11:identifier "006-MSG" ;
                                                rdfs:label "triggered by"@en ;
                                                skos:definition "p triggered by r =Def p is a response generation process & r is a message reception process & r is the causal antecedent that initiates p"@en ;
                                                skos:example "A response generation process triggered by receiving an email; an automated reply process triggered by message reception"@en .


#################################################################
#    Data Properties
#################################################################

###  http://ontology.naas.ai/messaging#hasContentLength
<http://ontology.naas.ai/messaging#hasContentLength> rdf:type owl:DatatypeProperty ;
                                                     rdfs:domain <http://ontology.naas.ai/messaging#MessageContent> ;
                                                     rdfs:range xsd:nonNegativeInteger ;
                                                     dc11:identifier "007-MSG" ;
                                                     rdfs:label "has content length"@en ;
                                                     skos:definition "c has content length n =Def c is message content & n is a non-negative integer representing the size measurement of c"@en ;
                                                     skos:example "A text message content has content length 160 characters; an email content has content length 1024 bytes"@en .


###  http://ontology.naas.ai/messaging#hasTextualContent
<http://ontology.naas.ai/messaging#hasTextualContent> rdf:type owl:DatatypeProperty ;
                                                      rdfs:domain <http://ontology.naas.ai/messaging#MessageContent> ;
                                                      rdfs:range xsd:string ;
                                                      dc11:identifier "008-MSG" ;
                                                      rdfs:label "has textual content"@en ;
                                                      skos:definition "c has textual content s =Def c is message content & s is a string & s is the textual representation of the information that c bears"@en ;
                                                      skos:example "An email content has textual content 'Hello World'; a chat message content has textual content 'See you tomorrow'"@en .


###  http://ontology.naas.ai/messaging#hasTimestamp
<http://ontology.naas.ai/messaging#hasTimestamp> rdf:type owl:DatatypeProperty ;
                                                 rdfs:domain [ owl:unionOf ( <http://ontology.naas.ai/messaging#MessageTransmissionProcess>
                                                                             <http://ontology.naas.ai/messaging#MessageReceptionProcess>
                                                                           )
                                                             ] ;
                                                 rdfs:range xsd:dateTime ;
                                                 dc11:identifier "009-MSG" ;
                                                 rdfs:label "has timestamp"@en ;
                                                 skos:definition "p has timestamp t =Def p is a messaging process & t is a dateTime & t represents the temporal instant at which p occurs"@en ;
                                                 skos:example "A message transmission process has timestamp 2024-01-15T10:30:00Z; a message reception process has timestamp 2024-01-15T10:30:01Z"@en .


#################################################################
#    Classes
#################################################################

###  http://ontology.naas.ai/messaging#Message
<http://ontology.naas.ai/messaging#Message> rdf:type owl:Class ;
                                            rdfs:subClassOf bfo:0000031 ,
                                                            [ rdf:type owl:Restriction ;
                                                              owl:onProperty <http://ontology.naas.ai/messaging#hasContent> ;
                                                              owl:someValuesFrom <http://ontology.naas.ai/messaging#MessageContent>
                                                            ] ;
                                            dc11:identifier "010-MSG" ;
                                            rdfs:label "message"@en ;
                                            skos:definition "b is a message =Def b is a generically dependent continuant that bears information content intended for transmission between agents"@en ;
                                            skos:example "An email message; a text message; a voice message; a video message"@en ;
                                            skos:scopeNote "Messages depend on some material substrate for their existence but can be copied across different substrates while maintaining their identity."@en .


###  http://ontology.naas.ai/messaging#MessageContent
<http://ontology.naas.ai/messaging#MessageContent> rdf:type owl:Class ;
                                                   rdfs:subClassOf bfo:0000031 ;
                                                   dc11:identifier "011-MSG" ;
                                                   rdfs:label "message content"@en ;
                                                   skos:definition "b is message content =Def b is a generically dependent continuant that is the information content entity constituting the semantic payload of a message"@en ;
                                                   skos:example "The textual content of an email; the semantic content of a spoken message; the informational payload of a data packet"@en .


###  http://ontology.naas.ai/messaging#MessageReceiverRole
<http://ontology.naas.ai/messaging#MessageReceiverRole> rdf:type owl:Class ;
                                                        rdfs:subClassOf bfo:0000023 ;
                                                        owl:disjointWith <http://ontology.naas.ai/messaging#MessageSenderRole> ;
                                                        dc11:identifier "012-MSG" ;
                                                        rdfs:label "message receiver role"@en ;
                                                        skos:definition "b is a message receiver role =Def b is a role that inheres in an agent & b is realized by processes in which that agent receives and processes transmitted information content"@en ;
                                                        skos:example "The role of being an email recipient; the role of being a chat participant who receives messages; the role of being a listener in a conversation"@en .


###  http://ontology.naas.ai/messaging#MessageReceptionProcess
<http://ontology.naas.ai/messaging#MessageReceptionProcess> rdf:type owl:Class ;
                                                            rdfs:subClassOf bfo:0000015 ,
                                                                            [ rdf:type owl:Restriction ;
                                                              owl:onProperty bfo:0000055 ;
                                                              owl:someValuesFrom <http://ontology.naas.ai/messaging#MessageReceiverRole>
                                                            ] ,
                                                                            [ rdf:type owl:Restriction ;
                                                              owl:onProperty <http://ontology.naas.ai/messaging#hasMessageInput> ;
                                                              owl:someValuesFrom <http://ontology.naas.ai/messaging#Message>
                                                            ] ;
                                                            owl:disjointWith <http://ontology.naas.ai/messaging#MessageTransmissionProcess> ,
                                                                             <http://ontology.naas.ai/messaging#ResponseGenerationProcess> ;
                                                            dc11:identifier "013-MSG" ;
                                                            rdfs:label "message reception process"@en ;
                                                            skos:definition "p is a message reception process =Def p is a process in which an agent with a message receiver role participates, and p has some message as input that the agent obtains and interprets"@en ;
                                                            skos:example "The process of receiving an email; the process of hearing a spoken message; the process of reading a text message"@en .


###  http://ontology.naas.ai/messaging#MessageSenderRole
<http://ontology.naas.ai/messaging#MessageSenderRole> rdf:type owl:Class ;
                                                      rdfs:subClassOf bfo:0000023 ;
                                                      dc11:identifier "014-MSG" ;
                                                      rdfs:label "message sender role"@en ;
                                                      skos:definition "b is a message sender role =Def b is a role that inheres in an agent & b is realized by processes in which that agent transmits information content to other agents"@en ;
                                                      skos:example "The role of being an email sender; the role of being a broadcaster; the role of being a speaker in a conversation"@en .


###  http://ontology.naas.ai/messaging#MessageTransmissionProcess
<http://ontology.naas.ai/messaging#MessageTransmissionProcess> rdf:type owl:Class ;
                                                               rdfs:subClassOf bfo:0000015 ,
                                                                               [ rdf:type owl:Restriction ;
                                                                 owl:onProperty bfo:0000055 ;
                                                                 owl:someValuesFrom <http://ontology.naas.ai/messaging#MessageSenderRole>
                                                               ] ,
                                                                               [ rdf:type owl:Restriction ;
                                                                 owl:onProperty <http://ontology.naas.ai/messaging#hasMessageOutput> ;
                                                                 owl:someValuesFrom <http://ontology.naas.ai/messaging#Message>
                                                               ] ;
                                                               owl:disjointWith <http://ontology.naas.ai/messaging#ResponseGenerationProcess> ;
                                                               dc11:identifier "015-MSG" ;
                                                               rdfs:label "message transmission process"@en ;
                                                               skos:definition "p is a message transmission process =Def p is a process in which an agent with a message sender role participates, and p has some message as output that the agent transmits to agents with receiver roles"@en ;
                                                               skos:example "The process of sending an email; the process of transmitting a radio signal; the process of speaking a message"@en .


###  http://ontology.naas.ai/messaging#ResponseGenerationProcess
<http://ontology.naas.ai/messaging#ResponseGenerationProcess> rdf:type owl:Class ;
                                                              rdfs:subClassOf bfo:0000015 ,
                                                                              [ rdf:type owl:Restriction ;
                                                                                owl:onProperty <http://ontology.naas.ai/messaging#triggeredBy> ;
                                                                                owl:someValuesFrom <http://ontology.naas.ai/messaging#MessageReceptionProcess>
                                                                              ] ;
                                                              dc11:identifier "016-MSG" ;
                                                              rdfs:label "response generation process"@en ;
                                                              skos:definition "p is a response generation process =Def p is a process in which an agent generates a response as a consequence of a message reception process"@en ;
                                                              skos:example "The process of composing a reply email; the process of generating an automated response; the process of responding in a conversation"@en ;
                                                              skos:scopeNote "Response generation processes are causally dependent on preceding message reception processes."@en .


#################################################################
#    General axioms
#################################################################

[ rdf:type owl:AllDisjointClasses ;
  owl:members ( <http://ontology.naas.ai/messaging#MessageTransmissionProcess>
                <http://ontology.naas.ai/messaging#MessageReceptionProcess>
                <http://ontology.naas.ai/messaging#ResponseGenerationProcess>
              )
] .


[ rdf:type owl:AllDisjointClasses ;
  owl:members ( <http://ontology.naas.ai/messaging#Message>
                <http://ontology.naas.ai/messaging#MessageContent>
              )
] .


