@prefix : <https://www.commoncoreontologies.org/TimeOntology/> .
@prefix obo: <http://purl.obolibrary.org/obo/> .
@prefix owl: <http://www.w3.org/2002/07/owl#> .
@prefix rdf: <http://www.w3.org/1999/02/22-rdf-syntax-ns#> .
@prefix xml: <http://www.w3.org/XML/1998/namespace> .
@prefix xsd: <http://www.w3.org/2001/XMLSchema#> .
@prefix cco: <https://www.commoncoreontologies.org/> .
@prefix rdfs: <http://www.w3.org/2000/01/rdf-schema#> .
@prefix skos: <http://www.w3.org/2004/02/skos/core#> .
@prefix dcterms: <http://purl.org/dc/terms/> .
@base <https://www.commoncoreontologies.org/TimeOntology> .

<https://www.commoncoreontologies.org/TimeOntology> rdf:type owl:Ontology ;
                                                                           owl:versionIRI <https://www.commoncoreontologies.org/2024-11-06/TimeOntology> ;
                                                                           owl:imports <https://www.commoncoreontologies.org/ExtendedRelationOntology> ;
                                                                           dcterms:license "BSD 3-Clause: https://github.com/CommonCoreOntology/CommonCoreOntologies/blob/master/LICENSE"@en ;
                                                                           dcterms:rights "CUBRC Inc., see full license."@en ;
                                                                           rdfs:comment "This ontology is designed to represent temporal regions and the relations that hold between them."@en ;
                                                                           rdfs:label "Time Ontology"@en ;
                                                                           owl:versionInfo "Version 2.0"@en .

#################################################################
#    Annotation properties
#################################################################

###  http://purl.org/dc/terms/rights
dcterms:rights rdf:type owl:AnnotationProperty .


###  https://www.commoncoreontologies.org/ont00001753
cco:ont00001753 rdf:type owl:AnnotationProperty .


###  https://www.commoncoreontologies.org/ont00001754
cco:ont00001754 rdf:type owl:AnnotationProperty .


###  https://www.commoncoreontologies.org/ont00001760
cco:ont00001760 rdf:type owl:AnnotationProperty .


#################################################################
#    Object Properties
#################################################################

###  https://www.commoncoreontologies.org/ont00001779
cco:ont00001779 rdf:type owl:ObjectProperty ;
                 owl:inverseOf cco:ont00001848 ;
                 rdfs:domain obo:BFO_0000038 ;
                 rdfs:range obo:BFO_0000148 ;
                 rdfs:label "has inside instant"@en ;
                 skos:definition "x has_inside_instant y iff x is an instance of One Dimensional Temporal Region and y is an instance of Temporal Instant and y is_inside_instant_of x."@en ;
                 cco:ont00001754 "J. F. Allen and J. A. G. M. Koomen. Planning using a temporal world model. In Proceedings of the 8th International Joint Conference on Artificial Intelligence (IJCAI-1983)  pages 741–747. Available at: https://www.ijcai.org/Proceedings/83-2/Papers/036.pdf"@en ;
                 cco:ont00001760 "https://www.commoncoreontologies.org/TimeOntology"^^xsd:anyURI .


###  https://www.commoncoreontologies.org/ont00001795
cco:ont00001795 rdf:type owl:ObjectProperty ;
                 rdfs:subPropertyOf cco:ont00001924 ;
                 owl:inverseOf cco:ont00001869 ;
                 rdfs:domain obo:BFO_0000202 ;
                 rdfs:range obo:BFO_0000202 ;
                 rdfs:label "has inside interval"@en ;
                 skos:definition "x has_inside_interval y iff x and y are both instances of Temporal Interval and y interval_during x."@en ;
                 cco:ont00001754 "J. F. Allen and J. A. G. M. Koomen. Planning using a temporal world model. In Proceedings of the 8th International Joint Conference on Artificial Intelligence (IJCAI-1983)  pages 741–747. Available at: https://www.ijcai.org/Proceedings/83-2/Papers/036.pdf"@en ;
                 cco:ont00001760 "https://www.commoncoreontologies.org/TimeOntology"^^xsd:anyURI .


###  https://www.commoncoreontologies.org/ont00001814
cco:ont00001814 rdf:type owl:ObjectProperty ;
                 rdfs:subPropertyOf cco:ont00001971 ;
                 rdfs:domain obo:BFO_0000202 ;
                 rdfs:range obo:BFO_0000202 ;
                 rdfs:label "interval finishes"@en ;
                 skos:definition "x interval_finishes y iff x and y are both instances of Temporal Interval and there exist instances of Temporal Instant v, w, and z such that v is the starting instant of x, w is the ending instant of both x and y, z is the starting instant of y, and z is before v."@en ;
                 cco:ont00001754 "J. F. Allen and J. A. G. M. Koomen. Planning using a temporal world model. In Proceedings of the 8th International Joint Conference on Artificial Intelligence (IJCAI-1983)  pages 741–747. Available at: https://www.ijcai.org/Proceedings/83-2/Papers/036.pdf"@en ;
                 cco:ont00001760 "https://www.commoncoreontologies.org/TimeOntology"^^xsd:anyURI .


###  https://www.commoncoreontologies.org/ont00001821
cco:ont00001821 rdf:type owl:ObjectProperty ;
                 rdfs:subPropertyOf cco:ont00001924 ;
                 owl:inverseOf cco:ont00001814 ;
                 rdfs:domain obo:BFO_0000202 ;
                 rdfs:range obo:BFO_0000202 ;
                 rdfs:label "interval finished by"@en ;
                 skos:definition "x interval_finished_by y iff x and y are both instances of Temporal Interval and y interval_finishes x."@en ;
                 cco:ont00001754 "J. F. Allen and J. A. G. M. Koomen. Planning using a temporal world model. In Proceedings of the 8th International Joint Conference on Artificial Intelligence (IJCAI-1983)  pages 741–747. Available at: https://www.ijcai.org/Proceedings/83-2/Papers/036.pdf"@en ;
                 cco:ont00001760 "https://www.commoncoreontologies.org/TimeOntology"^^xsd:anyURI .


###  https://www.commoncoreontologies.org/ont00001822
cco:ont00001822 rdf:type owl:ObjectProperty ,
                          owl:SymmetricProperty ;
                 rdfs:domain obo:BFO_0000202 ;
                 rdfs:range obo:BFO_0000202 ;
                 owl:propertyDisjointWith cco:ont00001862 ;
                 rdfs:label "interval equals"@en ;
                 skos:definition "x interval_equals y iff x and y are both instances of Temporal Interval and there exist instances of Temporal Instant w and z such that w is the starting instant of both x and y and z is the ending instant of both x and y."@en ;
                 cco:ont00001754 "J. F. Allen and J. A. G. M. Koomen. Planning using a temporal world model. In Proceedings of the 8th International Joint Conference on Artificial Intelligence (IJCAI-1983)  pages 741–747. Available at: https://www.ijcai.org/Proceedings/83-2/Papers/036.pdf"@en ;
                 cco:ont00001760 "https://www.commoncoreontologies.org/TimeOntology"^^xsd:anyURI .


###  https://www.commoncoreontologies.org/ont00001825
cco:ont00001825 rdf:type owl:ObjectProperty ;
                 owl:inverseOf cco:ont00001870 ;
                 rdfs:domain obo:BFO_0000202 ;
                 rdfs:range obo:BFO_0000202 ;
                 owl:propertyDisjointWith cco:ont00001862 ;
                 rdfs:label "interval overlaps"@en ;
                 skos:definition "x interval_overlaps y iff x and y are both instances of Temporal Interval and there exist instances of Temporal Instant u, v, w, z such that u is the starting instant of x, v is the ending instant of x, w is the starting instant of y, z is the ending instant of y, u is before w, w is before v, and v is before z."@en ;
                 cco:ont00001754 "J. F. Allen and J. A. G. M. Koomen. Planning using a temporal world model. In Proceedings of the 8th International Joint Conference on Artificial Intelligence (IJCAI-1983)  pages 741–747. Available at: https://www.ijcai.org/Proceedings/83-2/Papers/036.pdf"@en ;
                 cco:ont00001760 "https://www.commoncoreontologies.org/TimeOntology"^^xsd:anyURI .


###  https://www.commoncoreontologies.org/ont00001847
cco:ont00001847 rdf:type owl:ObjectProperty ;
                 rdfs:subPropertyOf cco:ont00001862 ;
                 owl:inverseOf cco:ont00001940 ;
                 rdfs:domain obo:BFO_0000202 ;
                 rdfs:range obo:BFO_0000202 ;
                 rdfs:label "interval is after"@en ;
                 skos:definition "x interval_is_after y iff x and y are both instances of Temporal Interval and y interval_is_before x."@en ;
                 cco:ont00001754 "J. F. Allen and J. A. G. M. Koomen. Planning using a temporal world model. In Proceedings of the 8th International Joint Conference on Artificial Intelligence (IJCAI-1983)  pages 741–747. Available at: https://www.ijcai.org/Proceedings/83-2/Papers/036.pdf"@en ;
                 cco:ont00001760 "https://www.commoncoreontologies.org/TimeOntology"^^xsd:anyURI .


###  https://www.commoncoreontologies.org/ont00001848
cco:ont00001848 rdf:type owl:ObjectProperty ;
                 rdfs:domain obo:BFO_0000148 ;
                 rdfs:range obo:BFO_0000038 ;
                 rdfs:label "is inside instant of"@en ;
                 skos:definition "x is_inside_instant of y iff x is an instance of Temporal Instant and y is an instance of One-Dimensional Temporal Region and there are instances of Temporal Instant w and z that are part of y and non-identical to x such that w precedes x and z is preceded by x."@en ;
                 cco:ont00001754 "J. F. Allen and J. A. G. M. Koomen. Planning using a temporal world model. In Proceedings of the 8th International Joint Conference on Artificial Intelligence (IJCAI-1983)  pages 741–747. Available at: https://www.ijcai.org/Proceedings/83-2/Papers/036.pdf"@en ;
                 cco:ont00001760 "https://www.commoncoreontologies.org/TimeOntology"^^xsd:anyURI .


###  https://www.commoncoreontologies.org/ont00001862
cco:ont00001862 rdf:type owl:ObjectProperty ;
                 rdfs:domain obo:BFO_0000202 ;
                 rdfs:range obo:BFO_0000202 ;
                 owl:propertyDisjointWith cco:ont00001870 ,
                                          cco:ont00001924 ,
                                          cco:ont00001971 ;
                 rdfs:label "interval disjoint"@en ;
                 skos:definition "x interval_disjoint y iff x and y are both instances of Temporal Interval and have no parts in common."@en ;
                 cco:ont00001754 "J. F. Allen and J. A. G. M. Koomen. Planning using a temporal world model. In Proceedings of the 8th International Joint Conference on Artificial Intelligence (IJCAI-1983)  pages 741–747. Available at: https://www.ijcai.org/Proceedings/83-2/Papers/036.pdf"@en ;
                 cco:ont00001760 "https://www.commoncoreontologies.org/TimeOntology"^^xsd:anyURI .


###  https://www.commoncoreontologies.org/ont00001869
cco:ont00001869 rdf:type owl:ObjectProperty ;
                 rdfs:subPropertyOf cco:ont00001971 ;
                 rdfs:domain obo:BFO_0000202 ;
                 rdfs:range obo:BFO_0000202 ;
                 rdfs:label "interval during"@en ;
                 skos:definition "x interval_during y iff x and y are both instances of Temporal Interval and there exist instances of Temporal Instant u, v, w, and z such that u is the starting instant of x, v is the ending instant of x, w is the starting instant of y, z is the ending instant of y, w is before u, and v is before z."@en ;
                 cco:ont00001754 "J. F. Allen and J. A. G. M. Koomen. Planning using a temporal world model. In Proceedings of the 8th International Joint Conference on Artificial Intelligence (IJCAI-1983)  pages 741–747. Available at: https://www.ijcai.org/Proceedings/83-2/Papers/036.pdf"@en ;
                 cco:ont00001760 "https://www.commoncoreontologies.org/TimeOntology"^^xsd:anyURI .


###  https://www.commoncoreontologies.org/ont00001870
cco:ont00001870 rdf:type owl:ObjectProperty ;
                 owl:inverseOf cco:ont00001825 ;
                 rdfs:domain obo:BFO_0000202 ;
                 rdfs:range obo:BFO_0000202 ;
                 rdfs:label "interval overlapped by"@en ;
                 skos:definition "x is_overlapped_by y iff x and y are both instances of Temporal Interval and y interval_overlaps x."@en ;
                 cco:ont00001754 "J. F. Allen and J. A. G. M. Koomen. Planning using a temporal world model. In Proceedings of the 8th International Joint Conference on Artificial Intelligence (IJCAI-1983)  pages 741–747. Available at: https://www.ijcai.org/Proceedings/83-2/Papers/036.pdf"@en ;
                 cco:ont00001760 "https://www.commoncoreontologies.org/TimeOntology"^^xsd:anyURI .


###  https://www.commoncoreontologies.org/ont00001875
cco:ont00001875 rdf:type owl:ObjectProperty ;
                 rdfs:subPropertyOf cco:ont00001924 ;
                 owl:inverseOf cco:ont00001923 ;
                 rdfs:domain obo:BFO_0000202 ;
                 rdfs:range obo:BFO_0000202 ;
                 rdfs:label "interval started by"@en ;
                 skos:definition "x interval_started_by y iff x and y are both instances of Temporal Interval and y interval_starts x."@en ;
                 cco:ont00001754 "J. F. Allen and J. A. G. M. Koomen. Planning using a temporal world model. In Proceedings of the 8th International Joint Conference on Artificial Intelligence (IJCAI-1983)  pages 741–747. Available at: https://www.ijcai.org/Proceedings/83-2/Papers/036.pdf"@en ;
                 cco:ont00001760 "https://www.commoncoreontologies.org/TimeOntology"^^xsd:anyURI .


###  https://www.commoncoreontologies.org/ont00001893
cco:ont00001893 rdf:type owl:ObjectProperty ;
                 owl:inverseOf cco:ont00001990 ;
                 rdf:type owl:TransitiveProperty ;
                 rdfs:domain obo:BFO_0000148 ;
                 rdfs:range obo:BFO_0000148 ;
                 rdfs:label "instant is after"@en ;
                 skos:definition "x instant_is_after y iff x and y are both instances of Temporal Instant and there exists some instance of Temporal Interval z such that y is the starting instant of z and x is the ending instant of z."@en ;
                 skos:scopeNote "'instant is after' is a primitive relationship. Informally, a temporal instant x is after some temporal instant y iff y precedes x."@en ;
                 cco:ont00001754 "J. F. Allen and J. A. G. M. Koomen. Planning using a temporal world model. In Proceedings of the 8th International Joint Conference on Artificial Intelligence (IJCAI-1983)  pages 741–747. Available at: https://www.ijcai.org/Proceedings/83-2/Papers/036.pdf"@en ;
                 cco:ont00001760 "https://www.commoncoreontologies.org/TimeOntology"^^xsd:anyURI .


###  https://www.commoncoreontologies.org/ont00001896
cco:ont00001896 rdf:type owl:ObjectProperty ;
                 rdfs:subPropertyOf cco:ont00001862 ;
                 rdf:type owl:IrreflexiveProperty ;
                 rdfs:domain obo:BFO_0000202 ;
                 rdfs:range obo:BFO_0000202 ;
                 rdfs:label "interval meets"@en ;
                 skos:definition "x interval_meets y iff x and y are both instances of Temporal Interval and there exists some instance of Temporal Instant z such that z is the ending instant of x and z is the starting instant of y."@en ;
                 cco:ont00001754 "J. F. Allen and J. A. G. M. Koomen. Planning using a temporal world model. In Proceedings of the 8th International Joint Conference on Artificial Intelligence (IJCAI-1983)  pages 741–747. Available at: https://www.ijcai.org/Proceedings/83-2/Papers/036.pdf"@en ;
                 cco:ont00001760 "https://www.commoncoreontologies.org/TimeOntology"^^xsd:anyURI .


###  https://www.commoncoreontologies.org/ont00001915
cco:ont00001915 rdf:type owl:ObjectProperty ;
                 rdfs:subPropertyOf cco:ont00001862 ;
                 rdf:type owl:IrreflexiveProperty ;
                 owl:inverseOf cco:ont00001896 ;
                 rdfs:domain obo:BFO_0000202 ;
                 rdfs:range obo:BFO_0000202 ;
                 rdfs:label "interval met by"@en ;
                 skos:definition "x interval_met_by y iff x and y are both instances of Temporal Interval and y interval_meets x."@en ;
                 cco:ont00001754 "J. F. Allen and J. A. G. M. Koomen. Planning using a temporal world model. In Proceedings of the 8th International Joint Conference on Artificial Intelligence (IJCAI-1983)  pages 741–747. Available at: https://www.ijcai.org/Proceedings/83-2/Papers/036.pdf"@en ;
                 cco:ont00001760 "https://www.commoncoreontologies.org/TimeOntology"^^xsd:anyURI .


###  https://www.commoncoreontologies.org/ont00001923
cco:ont00001923 rdf:type owl:ObjectProperty ;
                 rdfs:subPropertyOf cco:ont00001971 ;
                 rdfs:domain obo:BFO_0000202 ;
                 rdfs:range obo:BFO_0000202 ;
                 rdfs:label "interval starts"@en ;
                 skos:definition "x interval_starts y iff x and y are both instances of Temporal Interval and there exist instances of Temporal Instant v, w, and z such that v is the starting instant of both x and y, w is the ending instant of x, z is the ending instant of y and w is before z."@en ;
                 cco:ont00001754 "J. F. Allen and J. A. G. M. Koomen. Planning using a temporal world model. In Proceedings of the 8th International Joint Conference on Artificial Intelligence (IJCAI-1983)  pages 741–747. Available at: https://www.ijcai.org/Proceedings/83-2/Papers/036.pdf"@en ;
                 cco:ont00001760 "https://www.commoncoreontologies.org/TimeOntology"^^xsd:anyURI .


###  https://www.commoncoreontologies.org/ont00001924
cco:ont00001924 rdf:type owl:ObjectProperty ;
                 owl:inverseOf cco:ont00001971 ;
                 rdfs:domain obo:BFO_0000202 ;
                 rdfs:range obo:BFO_0000202 ;
                 rdfs:label "interval contains"@en ;
                 skos:definition "x interval_contains y iff x and y are both instances of Temporal Interval and there exist instances of Temporal Instant u, v, w, and z such that u is the starting instant of x, v is the ending instant of x, w is the starting instant of y, z is the ending instant of y, w is before or identical to u, and v is before or identical to z, and it is not the case that both w is identical to u and v is identical to z."@en ;
                 cco:ont00001754 "J. F. Allen and J. A. G. M. Koomen. Planning using a temporal world model. In Proceedings of the 8th International Joint Conference on Artificial Intelligence (IJCAI-1983)  pages 741–747. Available at: https://www.ijcai.org/Proceedings/83-2/Papers/036.pdf"@en ;
                 cco:ont00001760 "https://www.commoncoreontologies.org/TimeOntology"^^xsd:anyURI .


###  https://www.commoncoreontologies.org/ont00001940
cco:ont00001940 rdf:type owl:ObjectProperty ;
                 rdfs:subPropertyOf cco:ont00001862 ;
                 rdfs:domain obo:BFO_0000202 ;
                 rdfs:range obo:BFO_0000202 ;
                 rdfs:label "interval is before"@en ;
                 skos:definition "x interval_is_before y iff x and y are both instances of Temporal Interval and there exist instances of Temporal Instant w, z such that w is the ending instant of x and z is the starting instant of y and w is before z."@en ;
                 cco:ont00001754 "J. F. Allen and J. A. G. M. Koomen. Planning using a temporal world model. In Proceedings of the 8th International Joint Conference on Artificial Intelligence (IJCAI-1983)  pages 741–747. Available at: https://www.ijcai.org/Proceedings/83-2/Papers/036.pdf"@en ;
                 cco:ont00001760 "https://www.commoncoreontologies.org/TimeOntology"^^xsd:anyURI .


###  https://www.commoncoreontologies.org/ont00001971
cco:ont00001971 rdf:type owl:ObjectProperty ;
                 owl:inverseOf cco:ont00001924 ;
                 rdfs:domain obo:BFO_0000202 ;
                 rdfs:range obo:BFO_0000202 ;
                 rdfs:label "interval contained by"@en ;
                 skos:definition "x interval_contained_by y iff x and y are both instances of Temporal Interval and y interval_contains x."@en ;
                 cco:ont00001754 "J. F. Allen and J. A. G. M. Koomen. Planning using a temporal world model. In Proceedings of the 8th International Joint Conference on Artificial Intelligence (IJCAI-1983)  pages 741–747. Available at: https://www.ijcai.org/Proceedings/83-2/Papers/036.pdf"@en ;
                 cco:ont00001760 "https://www.commoncoreontologies.org/TimeOntology"^^xsd:anyURI .


###  https://www.commoncoreontologies.org/ont00001990
cco:ont00001990 rdf:type owl:ObjectProperty ,
                          owl:TransitiveProperty ;
                 rdfs:domain obo:BFO_0000148 ;
                 rdfs:range obo:BFO_0000148 ;
                 rdfs:label "instant is before"@en ;
                 skos:definition "x instant_is_before y iff x and y are both instances of Zero Dimensional Temporal Region and there exists some instance of Temporal Interval z such that x is the starting instant of z and y is the ending instant of z."@en ;
                 skos:scopeNote "'instant is before' is a primitive relationship. Informally, a temporal instant x is before some temporal instant y iff x precedes y."@en ;
                 cco:ont00001754 "J. F. Allen and J. A. G. M. Koomen. Planning using a temporal world model. In Proceedings of the 8th International Joint Conference on Artificial Intelligence (IJCAI-1983)  pages 741–747. Available at: https://www.ijcai.org/Proceedings/83-2/Papers/036.pdf"@en ;
                 cco:ont00001760 "https://www.commoncoreontologies.org/TimeOntology"^^xsd:anyURI .


#################################################################
#    Classes
#################################################################

###  https://www.commoncoreontologies.org/ont00000063
cco:ont00000063 rdf:type owl:Class ;
                 rdfs:subClassOf obo:BFO_0000038 ,
                                 [ rdf:type owl:Restriction ;
                                   owl:onProperty cco:ont00001924 ;
                                   owl:someValuesFrom cco:ont00001058
                                 ] ;
                 rdfs:comment "This is a defined class."@en ;
                 rdfs:label "Multi-Hour Temporal Interval"@en ;
                 skos:definition "A one-dimensional temporal region that is measured in Hours and spans at least one Hour."@en ;
                 cco:ont00001760 "https://www.commoncoreontologies.org/TimeOntology"^^xsd:anyURI .


###  https://www.commoncoreontologies.org/ont00000085
cco:ont00000085 rdf:type owl:Class ;
                 rdfs:subClassOf obo:BFO_0000202 ,
                                 [ rdf:type owl:Restriction ;
                                   owl:onProperty cco:ont00001869 ;
                                   owl:someValuesFrom cco:ont00001058
                                 ] ;
                 rdfs:label "Minute"@en ;
                 skos:definition "A Temporal Interval that is equal to sixty consecutive Seconds."@en ;
                 cco:ont00001754 "http://wordnetweb.princeton.edu/perl/webwn?s=minute" ;
                 cco:ont00001760 "https://www.commoncoreontologies.org/TimeOntology"^^xsd:anyURI .


###  https://www.commoncoreontologies.org/ont00000114
cco:ont00000114 rdf:type owl:Class ;
                 rdfs:subClassOf obo:BFO_0000203 ;
                 rdfs:label "Unix Temporal Instant"@en ;
                 skos:definition "A Temporal Instant as specified by the number of Seconds that have elapsed since the specified Epoch Time as described by an implementation of Unix Time."@en ;
                 cco:ont00001760 "https://www.commoncoreontologies.org/TimeOntology"^^xsd:anyURI .


###  https://www.commoncoreontologies.org/ont00000184
cco:ont00000184 rdf:type owl:Class ;
                 rdfs:subClassOf obo:BFO_0000202 ;
                 rdfs:label "Axial Rotation Period"@en ;
                 skos:definition "A Temporal Interval that is equal to the length of time required for a spinning Object to complete one rotation around its Axis of Rotation."@en ;
                 cco:ont00001760 "https://www.commoncoreontologies.org/TimeOntology"^^xsd:anyURI .


###  https://www.commoncoreontologies.org/ont00000211
cco:ont00000211 rdf:type owl:Class ;
                 rdfs:subClassOf obo:BFO_0000038 ,
                                 [ rdf:type owl:Restriction ;
                                   owl:onProperty cco:ont00001924 ;
                                   owl:someValuesFrom cco:ont00000800
                                 ] ;
                 rdfs:comment "This is a defined class."@en ;
                 rdfs:label "Multi-Day Temporal Interval"@en ;
                 skos:definition "A one-dimensional temporal region that is measured in Days and spans at least one Day."@en ;
                 cco:ont00001760 "https://www.commoncoreontologies.org/TimeOntology"^^xsd:anyURI .


###  https://www.commoncoreontologies.org/ont00000223
cco:ont00000223 rdf:type owl:Class ;
                 rdfs:subClassOf obo:BFO_0000203 ,
                                 [ rdf:type owl:Restriction ;
                                   owl:onProperty obo:BFO_0000132 ;
                                   owl:someValuesFrom cco:ont00000800
                                 ] ;
                 rdfs:label "Time of Day"@en ;
                 skos:definition "A Temporal Instant that is part of a Day."@en ;
                 cco:ont00001760 "https://www.commoncoreontologies.org/TimeOntology"^^xsd:anyURI .


###  https://www.commoncoreontologies.org/ont00000225
cco:ont00000225 rdf:type owl:Class ;
                 rdfs:subClassOf obo:BFO_0000202 ,
                                 [ rdf:type owl:Restriction ;
                                   owl:onProperty cco:ont00001869 ;
                                   owl:someValuesFrom cco:ont00000832
                                 ] ;
                 rdfs:label "Month"@en ;
                 skos:definition "A Temporal Interval that is based on the approximate length of time required for a Natural Satellite to complete one cycle of its rotational motion around its Primary Body."@en ;
                 skos:scopeNote "Unless otherwise specified, it is assumed that a Month is specified relative to the Rotational Motion of the Moon around the Earth. Earth Months are approximately equal to four consecutive Weeks or 30 consecutive Days."@en ;
                 cco:ont00001754 "http://wordnetweb.princeton.edu/perl/webwn?s=month" ;
                 cco:ont00001760 "https://www.commoncoreontologies.org/TimeOntology"^^xsd:anyURI .


###  https://www.commoncoreontologies.org/ont00000227
cco:ont00000227 rdf:type owl:Class ;
                 rdfs:subClassOf cco:ont00000674 ;
                 rdfs:comment "A Julian Year begins concurrently with January 1, ends concurrently with December 31, and has an average duration of exactly 365.25 Julian Days. Julian Years are typically indicated by prefixing a capital 'J' in front of the Year number, e.g. J2000.0 or J2018."@en ;
                 rdfs:label "Julian Year"@en ;
                 skos:definition "A Calendar Year in the Julian Calendar."@en ;
                 cco:ont00001760 "https://www.commoncoreontologies.org/TimeOntology"^^xsd:anyURI .


###  https://www.commoncoreontologies.org/ont00000259
cco:ont00000259 rdf:type owl:Class ;
                 rdfs:subClassOf cco:ont00000225 ;
                 rdfs:label "Calendar Month"@en ;
                 skos:definition "A Month that begins and ends concurrently with the Days specified by a Calendar System to be the first and last Days of the Month."@en ;
                 skos:example "January; February; March; April; May; June; July; August; September; October; November; December" ;
                 cco:ont00001760 "https://www.commoncoreontologies.org/TimeOntology"^^xsd:anyURI .


###  https://www.commoncoreontologies.org/ont00000329
cco:ont00000329 rdf:type owl:Class ;
                 rdfs:subClassOf obo:BFO_0000038 ,
                                 [ rdf:type owl:Restriction ;
                                   owl:onProperty cco:ont00001924 ;
                                   owl:someValuesFrom cco:ont00000225
                                 ] ;
                 rdfs:comment "This is a defined class."@en ;
                 rdfs:label "Multi-Month Temporal Interval"@en ;
                 skos:definition "A one-dimensional temporal region that is measured in Months and spans at least one Month."@en ;
                 cco:ont00001760 "https://www.commoncoreontologies.org/TimeOntology"^^xsd:anyURI .


###  https://www.commoncoreontologies.org/ont00000359
cco:ont00000359 rdf:type owl:Class ;
                 rdfs:subClassOf cco:ont00000223 ,
                                 [ rdf:type owl:Restriction ;
                                   owl:onProperty obo:BFO_0000132 ;
                                   owl:someValuesFrom cco:ont00000498
                                 ] ;
                 rdfs:label "Julian Date"@en ;
                 skos:definition "A Time of Day as specified according to the Julian Calendar using the Julian Date epoch."@en ;
                 cco:ont00001753 "JD" ;
                 cco:ont00001754 "https://www.defit.org/julian-date/" ;
                 cco:ont00001760 "https://www.commoncoreontologies.org/TimeOntology"^^xsd:anyURI .


###  https://www.commoncoreontologies.org/ont00000425
cco:ont00000425 rdf:type owl:Class ;
                 rdfs:subClassOf cco:ont00000674 ;
                 rdfs:comment "A Gregorian Year begins concurrently with January 1, ends concurrently with December 31, and has an average duration of exactly 365.2425 Gregorian Days. The Gregorian Year is based upon the vernal equinox year. Unless otherwise stated, instances of Calendar Year are assumed to be instances of Gregorian Year since the Gregorian Calendar is the most widely used civil Calendar System."@en ;
                 rdfs:label "Gregorian Year"@en ;
                 skos:definition "A Calendar Year in the Gregorian Calendar."@en ;
                 cco:ont00001760 "https://www.commoncoreontologies.org/TimeOntology"^^xsd:anyURI .


###  https://www.commoncoreontologies.org/ont00000435
cco:ont00000435 rdf:type owl:Class ;
                 rdfs:subClassOf cco:ont00000921 ;
                 rdfs:comment "A Gregorian Day is twenty-four Hours in duration."@en ;
                 rdfs:label "Gregorian Day"@en ;
                 skos:definition "A Calendar Day in the Gregorian Calendar."@en ;
                 cco:ont00001760 "https://www.commoncoreontologies.org/TimeOntology"^^xsd:anyURI .


###  https://www.commoncoreontologies.org/ont00000465
cco:ont00000465 rdf:type owl:Class ;
                 rdfs:subClassOf cco:ont00000223 ;
                 rdfs:comment """A Day begins at midnight GMT within the Modified Julian Date reference system. The Modified Julian Date (MJD) is related to the Julian Date (JD) by the formula:
MJD = JD - 2400000.5"""@en ;
                 rdfs:label "Modified Julian Date"@en ;
                 skos:definition "A Time of Day as specified according to the Julian Calendar using the Modified Julian Date epoch."@en ;
                 cco:ont00001753 "MJD" ;
                 cco:ont00001754 "http://aa.usno.navy.mil/data/docs/JulianDate.php" ;
                 cco:ont00001760 "https://www.commoncoreontologies.org/TimeOntology"^^xsd:anyURI .


###  https://www.commoncoreontologies.org/ont00000498
cco:ont00000498 rdf:type owl:Class ;
                 rdfs:subClassOf cco:ont00000921 ;
                 rdfs:comment "A Julian Day begins at noon Universal Time and is twenty-four Hours in duration."@en ;
                 rdfs:label "Julian Day"@en ;
                 skos:definition "A Calendar Day in the Julian Calendar."@en ;
                 cco:ont00001754 "https://www.defit.org/julian-date/" ;
                 cco:ont00001760 "https://www.commoncoreontologies.org/TimeOntology"^^xsd:anyURI .


###  https://www.commoncoreontologies.org/ont00000550
cco:ont00000550 rdf:type owl:Class ;
                 rdfs:subClassOf obo:BFO_0000202 ;
                 rdfs:label "Morning"@en ;
                 skos:definition "A Temporal Interval that consists of the temporal regions between when the sun dawns (approximately 6:00am) and reaches its apex (approximately 12:00pm)."@en ;
                 cco:ont00001760 "https://www.commoncoreontologies.org/TimeOntology"^^xsd:anyURI .


###  https://www.commoncoreontologies.org/ont00000619
cco:ont00000619 rdf:type owl:Class ;
                 rdfs:subClassOf obo:BFO_0000202 ,
                                 [ rdf:type owl:Restriction ;
                                   owl:onProperty cco:ont00001869 ;
                                   owl:someValuesFrom cco:ont00000225
                                 ] ;
                 rdfs:label "Week"@en ;
                 skos:definition "A Temporal Interval that is equal to seven consecutive Days."@en ;
                 cco:ont00001754 "http://wordnetweb.princeton.edu/perl/webwn?s=week" ;
                 cco:ont00001760 "https://www.commoncoreontologies.org/TimeOntology"^^xsd:anyURI .


###  https://www.commoncoreontologies.org/ont00000674
cco:ont00000674 rdf:type owl:Class ;
                 rdfs:subClassOf cco:ont00000832 ;
                 rdfs:label "Calendar Year"@en ;
                 skos:definition "A Year that begins and ends concurrently with the Days specified by a Calendar System to be the first and last Days of the Year."@en ;
                 cco:ont00001760 "https://www.commoncoreontologies.org/TimeOntology"^^xsd:anyURI .


###  https://www.commoncoreontologies.org/ont00000699
cco:ont00000699 rdf:type owl:Class ;
                 rdfs:subClassOf obo:BFO_0000202 ;
                 rdfs:label "Afternoon"@en ;
                 skos:definition "A Temporal Interval that consists of the temporal regions between when the sun is at its apex (approximately 12:00pm) and when it sets (approximately 6:00pm)."@en ;
                 cco:ont00001760 "https://www.commoncoreontologies.org/TimeOntology"^^xsd:anyURI .


###  https://www.commoncoreontologies.org/ont00000800
cco:ont00000800 rdf:type owl:Class ;
                 rdfs:subClassOf obo:BFO_0000202 ,
                                 [ rdf:type owl:Restriction ;
                                   owl:onProperty cco:ont00001869 ;
                                   owl:someValuesFrom cco:ont00000619
                                 ] ;
                 rdfs:label "Day"@en ;
                 skos:definition "A Temporal Interval that is equal to the approximate length of time required for an Astronomical Body to complete one rotation around its Rotational Axis as specified relative to a particular Temporal Reference System."@en ;
                 skos:scopeNote "Unless otherwise specified, a Day is assumed to be relative to the rotational motion of the Earth and is approximately equal to a twenty-four hour temporal region for which the start and end times are specified by the Temporal Reference System used."@en ;
                 cco:ont00001754 "http://wordnetweb.princeton.edu/perl/webwn?s=day" ;
                 cco:ont00001760 "https://www.commoncoreontologies.org/TimeOntology"^^xsd:anyURI .


###  https://www.commoncoreontologies.org/ont00000810
cco:ont00000810 rdf:type owl:Class ;
                 rdfs:subClassOf obo:BFO_0000038 ,
                                 [ rdf:type owl:Restriction ;
                                   owl:onProperty cco:ont00001924 ;
                                   owl:someValuesFrom cco:ont00000619
                                 ] ;
                 rdfs:comment "This is a defined class."@en ;
                 rdfs:label "Multi-Week Temporal Interval"@en ;
                 skos:definition "A one-dimensional temporal region that is measured in Weeks and spans at least one Week."@en ;
                 cco:ont00001760 "https://www.commoncoreontologies.org/TimeOntology"^^xsd:anyURI .


###  https://www.commoncoreontologies.org/ont00000832
cco:ont00000832 rdf:type owl:Class ;
                 rdfs:subClassOf obo:BFO_0000202 ,
                                 [ rdf:type owl:Restriction ;
                                   owl:onProperty cco:ont00001869 ;
                                   owl:someValuesFrom cco:ont00001088
                                 ] ;
                 rdfs:label "Year"@en ;
                 skos:definition "A Temporal Interval that is equal to the approximate length of time required for an Astronomical Body to complete one Orbital Revolution around its Primary Body as specified relative to a particular Temporal Reference System."@en ;
                 skos:scopeNote "Unless otherwise specified, a Year is assumed to be relative to the Orbiting of the Earth around the Sun and is approximately equal to 12 Months or 365 Days."@en ;
                 cco:ont00001754 "http://wordnetweb.princeton.edu/perl/webwn?s=year" ;
                 cco:ont00001760 "https://www.commoncoreontologies.org/TimeOntology"^^xsd:anyURI .


###  https://www.commoncoreontologies.org/ont00000921
cco:ont00000921 rdf:type owl:Class ;
                 rdfs:subClassOf cco:ont00000800 ;
                 rdfs:label "Calendar Day"@en ;
                 skos:definition "A Day that begins and ends concurrently with the Seconds specified by a Calendar System to be the first and last Seconds of the Day."@en ;
                 cco:ont00001760 "https://www.commoncoreontologies.org/TimeOntology"^^xsd:anyURI .


###  https://www.commoncoreontologies.org/ont00000992
cco:ont00000992 rdf:type owl:Class ;
                 rdfs:subClassOf obo:BFO_0000202 ,
                                 [ rdf:type owl:Restriction ;
                                   owl:onProperty cco:ont00001869 ;
                                   owl:someValuesFrom cco:ont00000085
                                 ] ;
                 rdfs:comment "The Second is used as the basic SI unit of time."@en ;
                 rdfs:label "Second"@en ;
                 skos:definition "A Temporal Interval that is equal to the duration of 9,192,631,770 periods of the radiation corresponding to the transition between the two hyperfine levels of the ground state of the cesium 133 atom."@en ;
                 cco:ont00001754 "https://physics.nist.gov/cuu/Units/second.html" ;
                 cco:ont00001760 "https://www.commoncoreontologies.org/TimeOntology"^^xsd:anyURI .


###  https://www.commoncoreontologies.org/ont00001023
cco:ont00001023 rdf:type owl:Class ;
                 rdfs:subClassOf cco:ont00000619 ;
                 rdfs:label "Calendar Week"@en ;
                 skos:definition "A Week that begins and ends concurrently with the Days specified by a Calendar System to be the first and last Days of the Week."@en ;
                 cco:ont00001754 "http://wordnetweb.princeton.edu/perl/webwn?s=calendar+week" ;
                 cco:ont00001760 "https://www.commoncoreontologies.org/TimeOntology"^^xsd:anyURI .


###  https://www.commoncoreontologies.org/ont00001058
cco:ont00001058 rdf:type owl:Class ;
                 rdfs:subClassOf obo:BFO_0000202 ,
                                 [ rdf:type owl:Restriction ;
                                   owl:onProperty cco:ont00001869 ;
                                   owl:someValuesFrom cco:ont00000800
                                 ] ;
                 rdfs:label "Hour"@en ;
                 skos:definition "A Temporal Interval that is equal to sixty consecutive Minutes."@en ;
                 cco:ont00001754 "http://wordnetweb.princeton.edu/perl/webwn?s=hour" ;
                 cco:ont00001760 "https://www.commoncoreontologies.org/TimeOntology"^^xsd:anyURI .


###  https://www.commoncoreontologies.org/ont00001088
cco:ont00001088 rdf:type owl:Class ;
                 rdfs:subClassOf obo:BFO_0000202 ;
                 rdfs:label "Decade"@en ;
                 skos:definition "A Temporal Interval that is equal to a period of ten consecutive Years."@en ;
                 cco:ont00001754 "http://wordnetweb.princeton.edu/perl/webwn?s=decade" ;
                 cco:ont00001760 "https://www.commoncoreontologies.org/TimeOntology"^^xsd:anyURI .


###  https://www.commoncoreontologies.org/ont00001110
cco:ont00001110 rdf:type owl:Class ;
                 rdfs:subClassOf obo:BFO_0000202 ;
                 rdfs:label "Evening"@en ;
                 skos:definition "A Temporal Interval that consists of the temporal regions between when the sun sets (approximately 6:00pm) and when people typically retire to sleep (approximately 9:00pm)."@en ;
                 cco:ont00001760 "https://www.commoncoreontologies.org/TimeOntology"^^xsd:anyURI .


###  https://www.commoncoreontologies.org/ont00001116
cco:ont00001116 rdf:type owl:Class ;
                 rdfs:subClassOf obo:BFO_0000203 ;
                 rdfs:label "Reference Time"@en ;
                 skos:altLabel "Epoch"@en ,
                               "Epoch Time"@en ,
                               "Reference Date"@en ;
                 skos:definition "A Temporal Instant specified as the origin for which other Temporal Regions are measured or identified."@en ;
                 cco:ont00001754 "https://en.wikipedia.org/wiki/Epoch_(reference_date)" ;
                 cco:ont00001760 "https://www.commoncoreontologies.org/TimeOntology"^^xsd:anyURI .


###  https://www.commoncoreontologies.org/ont00001154
cco:ont00001154 rdf:type owl:Class ;
                 rdfs:subClassOf obo:BFO_0000038 ,
                                 [ rdf:type owl:Restriction ;
                                   owl:onProperty cco:ont00001924 ;
                                   owl:someValuesFrom cco:ont00000992
                                 ] ;
                 rdfs:comment "This is a defined class."@en ;
                 rdfs:label "Multi-Second Temporal Interval"@en ;
                 skos:definition "A one-dimensional temporal region that is measured in Seconds and spans at least one Second."@en ;
                 cco:ont00001760 "https://www.commoncoreontologies.org/TimeOntology"^^xsd:anyURI .


###  https://www.commoncoreontologies.org/ont00001166
cco:ont00001166 rdf:type owl:Class ;
                 rdfs:subClassOf obo:BFO_0000038 ,
                                 [ rdf:type owl:Restriction ;
                                   owl:onProperty cco:ont00001924 ;
                                   owl:someValuesFrom cco:ont00000085
                                 ] ;
                 rdfs:comment "This is a defined class."@en ;
                 rdfs:label "Multi-Minute Temporal Interval"@en ;
                 skos:definition "A one-dimensional temporal region that is measured in Minutes and spans at least one Minute."@en ;
                 cco:ont00001760 "https://www.commoncoreontologies.org/TimeOntology"^^xsd:anyURI .


###  https://www.commoncoreontologies.org/ont00001204
cco:ont00001204 rdf:type owl:Class ;
                 rdfs:subClassOf obo:BFO_0000202 ;
                 rdfs:label "Night"@en ;
                 skos:definition "A Temporal Interval that consists of the temporal regions between when people typically retire to sleep (approximately 9:00pm) and when the sun dawns (approximately 6:00am)."@en ;
                 cco:ont00001760 "https://www.commoncoreontologies.org/TimeOntology"^^xsd:anyURI .


###  https://www.commoncoreontologies.org/ont00001206
cco:ont00001206 rdf:type owl:Class ;
                 rdfs:subClassOf obo:BFO_0000038 ,
                                 [ rdf:type owl:Restriction ;
                                   owl:onProperty cco:ont00001924 ;
                                   owl:someValuesFrom cco:ont00000832
                                 ] ;
                 rdfs:comment "This is a defined class."@en ;
                 rdfs:label "Multi-Year Temporal Interval"@en ;
                 skos:definition "A one-dimensional temporal region that is measured in Years and spans at least one Year."@en ;
                 cco:ont00001760 "https://www.commoncoreontologies.org/TimeOntology"^^xsd:anyURI .


###  Generated by the OWL API (version 4.5.29) https://github.com/owlcs/owlapi
