@prefix owl: <http://www.w3.org/2002/07/owl#> .
@prefix dc11: <http://purl.org/dc/elements/1.1/> .
@prefix dc: <http://purl.org/dc/terms/> .
@prefix rdf: <http://www.w3.org/1999/02/22-rdf-syntax-ns#> .
@prefix rdfs: <http://www.w3.org/2000/01/rdf-schema#> .
@prefix xsd: <http://www.w3.org/2001/XMLSchema#> .
@prefix skos: <http://www.w3.org/2004/02/skos/core#> .
@prefix bfo: <http://purl.obolibrary.org/obo/> .
@prefix cco: <https://www.commoncoreontologies.org/> .
@prefix abi: <http://ontology.naas.ai/abi/> .

#################################################################
#    Classes
#################################################################

abi:Country a owl:Class ;
    rdfs:subClassOf cco:ont00000472 ;
    rdfs:label "Country" ;
    skos:definition "A Geospatial Region that is a distinct territorial body or political entity recognized as an independent nation." ;
    skos:example "United States, France, Japan" ;
    rdfs:comment "A country is a distinct region with recognized boundaries and political governance, making it a suitable subclass of cco:GeospatialRegion." .

abi:Address rdf:type owl:Class ;
    rdfs:subClassOf cco:ont00000686 ;
    rdfs:label "Address" ;
    skos:definition "A Designative Information Content Entity that consists of a structured string of characters used to identify the location of an entity, typically including elements such as street name, number, city, region, and postal code." ;
    skos:example "123 Main St, New York, NY 10001" ;
    rdfs:comment "An Address is a structured string of characters used to identify the location of an entity, typically including elements such as street name, number, city, region, and postal code." .

abi:ZIPCode rdf:type owl:Class ;
    rdfs:subClassOf cco:ont00000686 ;
    rdfs:label "ZIP Code" ;
    skos:definition "A Designative Information Content Entity that consists of a string of characters used to identify a postal delivery area." ;
    skos:example "92130" ;
    rdfs:comment "A ZIP Code is a structured string of characters used to identify a postal delivery area for mail sorting and delivery purposes." .

#################################################################
#    Datatype Properties
#################################################################

abi:country_code a owl:DatatypeProperty ;
    rdfs:domain abi:Country ;
    rdfs:range xsd:string ;
    rdfs:label "Country Code" ;
    skos:definition "The ISO 3166-1 alpha-2 code for the country." ;
    skos:example "US, FR, JP" .
