@prefix owl: <http://www.w3.org/2002/07/owl#> .
@prefix dc11: <http://purl.org/dc/elements/1.1/> .
@prefix dc: <http://purl.org/dc/terms/> .
@prefix rdf: <http://www.w3.org/1999/02/22-rdf-syntax-ns#> .
@prefix rdfs: <http://www.w3.org/2000/01/rdf-schema#> .
@prefix xsd: <http://www.w3.org/2001/XMLSchema#> .
@prefix skos: <http://www.w3.org/2004/02/skos/core#> .
@prefix bfo: <http://purl.obolibrary.org/obo/> .
@prefix cco: <https://www.commoncoreontologies.org/> .
@prefix abi: <http://ontology.naas.ai/abi/> .

<http://ontology.naas.ai/abi/linkedin.ttl> rdf:type owl:Ontology ;
                                        owl:imports <> ;
                                        owl:versionIRI <https://github.com/jupyter-naas/abi/tree/cli/src/ontologies/application-level/linkedin.ttl> ;
                                        dc11:contributor "Jeremy Ravenel" , "Maxime Jublou" , "Florent Ravenel" ;
                                        dc:description "Application ontology for LinkedIn."@en ;
                                        dc:license "" ;
                                        dc:title "LinkedIn Application Ontology" .

#################################################################
#    Classes
#################################################################

abi:LinkedInPage a owl:Class ;
    rdfs:subClassOf cco:ont00001069 ; # Representational Information Content Entity
    rdfs:label "LinkedIn Page" ;
    skos:definition "A LinkedIn page that represents an entity's presence on LinkedIn, containing information specific to that entity type such as professional details, organizational information, or educational programs." ;
    skos:example "A LinkedIn page could be a profile page showing work experience, a company page with job postings, or a school page highlighting academic programs." ;
    rdfs:comment "A LinkedIn page must be registered in https://www.linkedin.com/" .

abi:LinkedInProfilePage a owl:Class ;
    rdfs:subClassOf abi:LinkedInPage ;
    rdfs:label "LinkedIn Profile Page" ;
    skos:definition "A LinkedIn profile page that includes information such as a person's professional history, skills, and endorsements, representing the individual's professional identity on the web." ;
    skos:example "John Doe's LinkedIn profile page, which lists his work experience at various companies, skills such as programming and data analysis, and endorsements from colleagues." ;
    rdfs:comment "A LinkedIn profile page must be registered in https://www.linkedin.com/in/" .

abi:LinkedInCompanyPage a owl:Class ;
    rdfs:subClassOf abi:LinkedInPage ;
    rdfs:label "LinkedIn Company Page" ;
    skos:definition "A LinkedIn company page that includes information such as the company's overview, products/services, job postings, and updates, representing the organization's professional presence on LinkedIn." ;
    skos:example "Microsoft's LinkedIn company page, which showcases their company information, latest news, job opportunities, and employee insights." ;
    rdfs:comment "A LinkedIn company page must be registered in https://www.linkedin.com/company/" .

abi:LinkedInSchoolPage a owl:Class ;
    rdfs:subClassOf abi:LinkedInPage ;
    rdfs:label "LinkedIn School Page" ;
    skos:definition "A LinkedIn school page that includes information about the school's programs, faculty, students, and events, representing the educational institution's professional presence on LinkedIn." ;
    rdfs:comment "A LinkedIn school page must be registered in https://www.linkedin.com/school/" .

#################################################################
#    Object Properties
#################################################################

abi:hasLinkedInPage a owl:ObjectProperty ;
    rdfs:domain [ rdf:type owl:Class ;
                  owl:unionOf ( cco:ont00001180
                               cco:ont00001262
                             )
                ] ;
    rdfs:range abi:LinkedInPage ;
    owl:inverseOf abi:isLinkedInPageOf ;
    rdfs:label "has linkedin page"@en ;
    skos:definition "Relates an entity to its LinkedIn page."@en ;
    skos:example "John Doe's LinkedIn profile page, which lists his work experience at various companies, skills such as programming and data analysis, and endorsements from colleagues."@en .

abi:isLinkedInPageOf a owl:ObjectProperty ;
    rdfs:domain abi:LinkedInPage ;
    rdfs:range [ rdf:type owl:Class ;
                 owl:unionOf ( cco:ont00001180
                              cco:ont00001262
                            )
               ] ;
    owl:inverseOf abi:hasLinkedInPage ;
    rdfs:label "is linkedin page of"@en ;
    skos:definition "Relates a LinkedIn page to the entity it represents."@en ;
    skos:example "A LinkedIn profile page that represents John Doe's professional presence."@en .

#################################################################
#    Data properties
#################################################################

abi:linkedin_id a owl:DatatypeProperty ;
    rdfs:domain abi:LinkedInPage ;
    rdfs:range xsd:string ;
    rdfs:label "LinkedIn ID"@en ;
    skos:definition "The ID of the LinkedIn page."@en ;
    skos:example "The unique ID of John Doe's LinkedIn profile page is 'ACoAAAa5py0Bzrp5_7OmHIsNP6xxxxxxxx'."@en .

abi:linkedin_url a owl:DatatypeProperty ;
    rdfs:domain abi:LinkedInPage ;
    rdfs:range xsd:string ;
    rdfs:label "LinkedIn URL"@en ;
    skos:definition "The URL of the LinkedIn page. It uses the LinkedIn ID as a unique identifier."@en ;
    skos:example "The URL of John Doe's LinkedIn profile page is 'https://www.linkedin.com/in/ACoAAAa5py0Bzrp5_7OmHIsNP6xxxxxxxx'."@en .

abi:linkedin_public_id a owl:DatatypeProperty ;
    rdfs:domain abi:LinkedInPage ;
    rdfs:range xsd:string ;
    rdfs:label "LinkedIn Public ID"@en ;
    skos:definition "The public ID of the LinkedIn page. It might change over time."@en ;
    skos:example "The public ID of John Doe's LinkedIn profile page is 'johndoe'."@en .

abi:linkedin_public_url a owl:DatatypeProperty ;
    rdfs:domain abi:LinkedInPage ;
    rdfs:range xsd:string ;
    rdfs:label "LinkedIn Public URL"@en ;
    skos:definition "The public URL of the LinkedIn page. It uses the LinkedIn Public ID as identifier."@en ;
    skos:example "The public URL of John Doe's LinkedIn profile page is 'https://www.linkedin.com/in/johndoe'."@en .



