@prefix owl: <http://www.w3.org/2002/07/owl#> .
@prefix dc11: <http://purl.org/dc/elements/1.1/> .
@prefix dc: <http://purl.org/dc/terms/> .
@prefix rdf: <http://www.w3.org/1999/02/22-rdf-syntax-ns#> .
@prefix rdfs: <http://www.w3.org/2000/01/rdf-schema#> .
@prefix xsd: <http://www.w3.org/2001/XMLSchema#> .
@prefix skos: <http://www.w3.org/2004/02/skos/core#> .
@prefix bfo: <http://purl.obolibrary.org/obo/> .
@prefix cco: <https://www.commoncoreontologies.org/> .
@prefix abi: <http://ontology.naas.ai/abi/> .

<http://ontology.naas.ai/abi/OrganizationOntology> rdf:type owl:Ontology ;
    owl:imports <https://www.commoncoreontologies.org/AgentOntology> ;
    owl:versionIRI <https://github.com/jupyter-naas/abi/tree/cli/src/ontologies/domain-level/OrganizationOntology.ttl> ;
    dc11:contributor "Jeremy Ravenel" , "Maxime Jublou" , "Florent Ravenel" ;
    dc:description "Domain ontology for organizations."@en ;
    dc:license "" ;
    dc:title "Organization Ontology" .

#################################################################
#    Classes
#################################################################

abi:BusinessDomain a owl:Class ;
    rdfs:subClassOf cco:ont00000958 ;
    rdfs:label "Business Domain" ;
    skos:definition "A Business Domain is an Information Content Entity that represents a specific area of expertise or activity within an organization, characterized by distinct processes, goals, and practices." ;
    skos:example "Marketing, Sales, Engineering, etc." ;
    rdfs:comment "Business Domains are specialized areas within an organization that focus on specific business functions or activities." .

abi:Industry a owl:Class ;
    rdfs:subClassOf cco:ont00000958 ;
    rdfs:label "Industry" ;
    skos:definition "An Industry is an Information Content Entity that represents a broad category of businesses or organizations that produce similar products or services within a market." ;
    skos:example "Technology, Finance, Healthcare, etc." ;
    rdfs:comment "Industries encompass the collective market activities and economic sector of companies producing similar goods or services." .

abi:StaffRange a owl:Class ;
    rdfs:subClassOf cco:ont00000958 ;
    rdfs:label "Staff Range"@en ;
    skos:definition "A Staff Range is an Information Content Entity that represents a range of staff size within an organization." ;
    skos:example "Micro Team, Small Team, Medium Team, Large Team, Enterprise Team." ;
    rdfs:comment "Staff Ranges are used to categorize the size of an organization's staff." .

#################################################################
#    Object Properties
#################################################################

abi:hasStaffRange a owl:ObjectProperty ;
    rdfs:subPropertyOf bfo:BFO_0000115 ;
    rdfs:domain cco:ont00000647 ; # Organization
    rdfs:range abi:StaffRange ;
    rdfs:label "has staff range"@en ;
    skos:definition "A relation between an organization and its staff range."@en ;
    rdfs:comment "This property captures the relationship between an organization and the size of its staff, which is crucial for understanding the organizational structure and capacity." .

abi:hasBusinessDomain a owl:ObjectProperty ;
    rdfs:subPropertyOf bfo:BFO_0000115 ;
    rdfs:domain cco:ont00000647 ; # Organization
    rdfs:range abi:BusinessDomain ;
    rdfs:label "has business domain" ;
    skos:definition "Relates an Organization to the Business Domain it operates in, indicating the specific areas of expertise or activity within the organization." ;
    rdfs:comment "This property links an organization to its internal areas of specialization and activity." .

abi:operatesInIndustry a owl:ObjectProperty ;
    rdfs:subPropertyOf bfo:BFO_0000115 ;
    rdfs:domain cco:ont00000647 ; # Organization
    rdfs:range abi:Industry ;
    rdfs:label "operates in industry" ;
    skos:definition "Relates an Organization to the Industry in which it operates, indicating the broader market category of its products or services." ;
    rdfs:comment "This property connects an organization to the wider economic sector it belongs to, based on its market activities." .

#################################################################
#    Data Properties
#################################################################

abi:logo a owl:DatatypeProperty ;
    rdfs:domain cco:ont00000647 ; # Organization
    rdfs:range xsd:string ;
    rdfs:label "logo" ;
    skos:definition "The URL of the logo of the organization." ;
    rdfs:comment "The URL of the logo of the organization." .

#################################################################
#    Individuals
#################################################################

abi:Solopreneur a abi:StaffRange ;
    rdfs:label "Solopreneur" ;
    skos:definition "An individual entrepreneur or freelancer operating alone (0-1 employees)" .

abi:MicroTeam a abi:StaffRange ;
    rdfs:label "Micro Team" ;
    skos:definition "A small team consisting of 2 to 10 members" .

abi:SmallCompany a abi:StaffRange ;
    rdfs:label "Small Company" ;
    skos:definition "A small company with 11 to 50 employees" .

abi:MediumCompany a abi:StaffRange ;
    rdfs:label "Medium Company" ;
    skos:definition "A medium-sized company with 51 to 200 employees" .

abi:LargeCompany a abi:StaffRange ;
    rdfs:label "Large Company" ;
    skos:definition "A large company with 201 to 500 employees" .

abi:EnterpriseLevelCompany a abi:StaffRange ;
    rdfs:label "Enterprise Level" ;
    skos:definition "An enterprise-level organization with 501 to 1000 employees" .

abi:MajorCorporation a abi:StaffRange ;
    rdfs:label "Major Corporation" ;
    skos:definition "A large corporation with 1001 to 5000 employees" .

abi:GlobalCorporation a abi:StaffRange ;
    rdfs:label "Global Corporation" ;
    skos:definition "A global corporation with 5001 to 10000 employees" .

abi:MegaCorporation a abi:StaffRange ;
    rdfs:label "Mega Corporation" ;
    skos:definition "A massive corporation with more than 10000 employees" .